Control/Monad/Class/MonadFail.v
@@ -1,8 +1,8 @@
 Require Export Control.Monad.
 
-(** A monad which models a computation that can fail. If a computation
-    fails, any later computations that depend on it also fail, as
-    exhibited by teh law [bind_fail_l]. *)
+(** A monad which models computations that can fail. If a computation
+    fails, any later computation that depends on it also fails, as
+    exhibited by the law [bind_fail_l]. *)
 Class MonadFail (M : Type -> Type) (inst : Monad M) : Type :=
 {
     fail : forall {A :  Type}, M A;
@@ -21,11 +21,22 @@ Variables M : Type -> Type.
 Variable instM : Monad M.
 Variable instMF : MonadFail M instM.
 
-Definition mfilter {A : Type} (f : A -> bool) (ma : M A) : M A :=
-  ma >>= fun a : A => if f a then pure a else fail.
+(** We can "filter" a computation by running it and then wrapping
+    values that satisfy the given boolean predicate in [pure] and
+    turning the ones that don't into [fail]s. *)
+Definition mfilter {A : Type} (p : A -> bool) (ma : M A) : M A :=
+  ma >>= fun a : A => if p a then pure a else fail.
 
+(** Using [mfilter], we can partition a computation into two computations
+    that satisfy and don't satisfy a predicate [p], respectively. *)
 Definition mpartition {A : Type} (p : A -> bool) (ma : M A) : M A * M A :=
   (mfilter p ma, mfilter (p .> negb) ma).
+
+(** We can turn an optional value of type [A] into a computation by
+    treating [Some] as success and [None] as failure. Thnaks to this,
+    we can turn computations that return [option A] into ones that
+    return just [A]. We can use this for mapping partial functions
+    over our computations. *)
 
 Definition fromOption {A : Type} (oa : option A) : M A :=
 match oa with
@@ -35,6 +46,12 @@ end.
 
 Definition mcatOptions {A : Type} (x : M (option A)) : M A :=
   x >>= fromOption.
+
+Definition mmapOption {A B : Type} (f : A -> option B) (x : M A) : M B :=
+  mcatOptions (fmap f x).
+
+(** Similarly, we can split a computation that returns a sum into two
+    computations that return the left and right component of the sum. *)
 
 Definition sum_left {A B : Type} (x : A + B) : option A :=
 match x with
@@ -56,9 +73,6 @@ Definition mrights {A B : Type} (x : M (A + B)) : M B :=
 
 Definition mpartitionSums {A B : Type} (x : M (A + B)) : M A * M B :=
   (mlefts x, mrights x).
-
-Definition mmapOption {A B : Type} (f : A -> option B) (x : M A) : M B :=
-  mcatOptions (fmap f x).
 
 End MonadFailFuns.
 
