Control/Monad/Class/MonadNondet.v
@@ -1,9 +1,9 @@
 Require Export Control.Monad.Class.MonadFail.
 Require Export Control.Monad.Class.MonadAlt.
 
-(** Nondeterminism monad. We have failure and nondeterministic choice.
-    The laws can be summarized by saying that if we can choose, we
-    don't choose failure. *)
+(** A monad that represents nondeterministic computations, i.e. ones that can
+    [fail] and make choices. The laws can be summarized by saying that if we
+    can choose, we don't choose failure. *)
 Class MonadNondet (M : Type -> Type) (inst : Monad M) : Type :=
 {
     instF :> MonadFail M inst;
