Control/Monad/Class/MonadReader.v
@@ -1,4 +1,5 @@
 Require Export Control.Monad.
+Require Import Control.Monad.Trans.
 
 (** Reader monad that provides access to some kind of environment.
     We can ask for the contents of the environment and if we ask
@@ -30,10 +31,7 @@ End MonadReader_funs.
 
 (** Interestingly, we can prove that if the base monad [M] has an instance
     of [MonadReader], then a monad transformer fed with [M] also has an
-    instance of [MonadReader]. This is quite impossible with the other
-    classes. *)
-Require Import Control.Monad.Trans.
-
+    instance of [MonadReader]. This is impossible with the other classes. *)
 Instance MonadReader_MonadTrans
   (T : (Type -> Type) -> Type -> Type) (instT : MonadTrans T)
   (M : Type -> Type) (instM : Monad M)
