Control/Monad/Class/MonadStateNondet.v
@@ -2,7 +2,11 @@ Require Export Control.Monad.Class.MonadNondet.
 Require Export Control.Monad.Class.MonadState.
 
 (** A monad that models both nondeterministic and stateful computations.
-    
+    The law [seq_fail_r] says that eventual failure makes the whole
+    computation fail. [bind_choose_r] says that if a choice depends on
+    a previous computation, it can be expressed as a more complicated
+    choice. They can probably be summed up by saying that the state is
+    local to each branch of nondeterminism.
 *)
 Class MonadStateNondet
   (S : Type) (M : Type -> Type) (inst : Monad M) : Type :=
